formal-proofs/theories/lib/concurrent_linked_list/list_spec.v
@@ -7,9 +7,12 @@ Record listSpec Σ `{!heapG Σ} {impl: segmentInterface}
        (segment_spec: segmentSpec Σ impl) :=
   ListSpec {
       list_name: Type;
-      is_concurrentLinkedList: namespace -> list_name -> iProp Σ;
-      is_concurrentLinkedList_persistent N γ:
-        Persistent (is_concurrentLinkedList N γ);
+      is_concurrentLinkedList:
+        namespace ->
+        linkedListNode_parameters _ _ (linkedListNode_base _ _ segment_spec) ->
+        list_name -> iProp Σ;
+      is_concurrentLinkedList_persistent N p γ:
+        Persistent (is_concurrentLinkedList N p γ);
       segment_in_list
         (γ: list_name)
         (γs: linkedListNode_name _ _ (linkedListNode_base _ _ segment_spec))
@@ -26,23 +29,23 @@ Record listSpec Σ `{!heapG Σ} {impl: segmentInterface}
       findSegment: val;
       moveForward: val;
       onSlotCleaned: val;
-      newList_spec N (k: nat):
+      newList_spec N p (k: nat):
         {{{ ⌜k > 0⌝ ∧ initialization_requirements _ _ segment_spec }}}
           newList #k
-        {{{ γ ℓ, RET #ℓ; is_concurrentLinkedList N γ ∗
+        {{{ γ ℓ, RET #ℓ; is_concurrentLinkedList N p γ ∗
                         [∗ list] i ∈ seq 0 k,
                             pointer_location γ (ℓ +ₗ (i: nat)) 0
         }}};
-      findSegment_spec N γ γs' (start_id id: nat) v:
-        {{{ is_concurrentLinkedList N γ ∗ segment_in_list γ γs' start_id v }}}
+      findSegment_spec N p γ γs' (start_id id: nat) v:
+        {{{ is_concurrentLinkedList N p γ ∗ segment_in_list γ γs' start_id v }}}
           findSegment v #id
         {{{ (v': val) (id': nat), RET (SOMEV v');
           (∃ γs, segment_in_list γ γs id' v')
           ∗ ⌜(start_id ≤ id' ∧ id ≤ id')%nat⌝
           ∗ ∀ i, (⌜max start_id id ≤ i < id'⌝)%nat -∗ segment_is_cancelled γ i
         }}};
-      moveForward_spec N γ γs (ℓ: loc) id v:
-        is_concurrentLinkedList N γ -∗
+      moveForward_spec N p γ γs (ℓ: loc) id v:
+        is_concurrentLinkedList N p γ -∗
         segment_in_list γ γs id v -∗
         <<< ∀ id', ▷ pointer_location γ ℓ id' >>>
           moveForward #ℓ v @ ⊤ ∖ ↑N
@@ -50,12 +53,12 @@ Record listSpec Σ `{!heapG Σ} {impl: segmentInterface}
                               else ▷ pointer_location γ ℓ id'
                                    ∗ segment_is_cancelled γ id,
             RET #r >>>;
-      cleanPrev_spec N γ γs id ptr:
-        {{{ is_concurrentLinkedList N γ ∗ segment_in_list γ γs id ptr }}}
+      cleanPrev_spec N p γ γs id ptr:
+        {{{ is_concurrentLinkedList N p γ ∗ segment_in_list γ γs id ptr }}}
           cleanPrev ptr
         {{{ RET #(); True }}};
-      onSlotCleaned_spec N Ψ γ γs id p:
-        is_concurrentLinkedList N γ -∗
+      onSlotCleaned_spec N pars Ψ γ γs id p:
+        is_concurrentLinkedList N pars γ -∗
         segment_in_list γ γs id p -∗
         <<< (∀ n, segment_content _ _ segment_spec γs n ==∗
             Ψ ∗ ∃ n', ⌜(n = S n')%nat⌝ ∧
@@ -67,9 +70,9 @@ Record listSpec Σ `{!heapG Σ} {impl: segmentInterface}
           ! #ℓ @ ⊤
         <<< ∃ γs p, pointer_location γ ℓ id ∗ segment_in_list γ γs id p,
             RET p >>>;
-      access_segment N (known_is_removed: bool) E γ γs id ptr:
+      access_segment N pars (known_is_removed: bool) E γ γs id ptr:
         ↑N ⊆ E ->
-        is_concurrentLinkedList N γ -∗
+        is_concurrentLinkedList N pars γ -∗
         segment_in_list γ γs id ptr -∗
         (if known_is_removed then segment_is_cancelled γ id else True) -∗
         |={E, E ∖ ↑N}=> ∃ n, ⌜known_is_removed = false ∨ n = 0⌝ ∧
